ReactorModel/Execution/Theorems/State.lean
@@ -6,13 +6,15 @@ open Classical Reactor
 
 namespace Execution.State
 
-variable [Hierarchical α] {s s₁ s₂ : State α}
+variable {s s₁ s₂ : State α}
 
-theorem input_congr (hr : s₁.rtr = s₂.rtr := by rfl) (ht : s₁.tag = s₂.tag := by rfl) :
+theorem input_congr
+    [Hierarchical α] (hr : s₁.rtr = s₂.rtr := by rfl) (ht : s₁.tag = s₂.tag := by rfl) :
     s₁.input i = s₂.input i := by
   simp [input, input.restriction, hr, ht]
 
-theorem output_congr (hr : s₁.rtr = s₂.rtr := by rfl) (ht : s₁.tag = s₂.tag := by rfl) :
+theorem output_congr
+    [Hierarchical α] (hr : s₁.rtr = s₂.rtr := by rfl) (ht : s₁.tag = s₂.tag := by rfl) :
     s₁.output i = s₂.output i := by
   simp [output, input_congr hr ht, hr]
 
@@ -25,11 +27,11 @@ theorem record_preserves_tag (s : State α) (rcn : ID) : (s.record rcn).tag = s.
 theorem record_preserves_events (s : State α) (rcn : ID) : (s.record rcn).events = s.events :=
   rfl
 
-theorem record_progress_eq (s : State α) (rcn₁ rcn₂ : ID) :
+theorem record_progress_eq (s : State α) (rcn : ID) :
     (s.record rcn).progress = s.progress.insert rcn :=
   rfl
 
-theorem record_preserves_output (s : State α) (rcn₁ rcn₂ : ID) :
+theorem record_preserves_output [Hierarchical α] (s : State α) (rcn₁ rcn₂ : ID) :
     (s.record rcn₁).output rcn₂ = s.output rcn₂ :=
   output_congr (s.record_preserves_rtr _) (s.record_preserves_tag _)
 
@@ -58,6 +60,8 @@ theorem schedule_ne_comm {s : State α} {i₁ i₂ : ID} {t₁ t₂ : Time} {v�
     (s.schedule i₁ t₁ v₁).schedule i₂ t₂ v₂ = (s.schedule i₂ t₂ v₂).schedule i₁ t₁ v₁ := by
   simp [schedule]
   apply Partial.update_ne_comm _ h
+
+variable [Hierarchical α]
 
 theorem Allows.«def» :
     (s.Allows i) ↔ (i ∈ s.rtr[.rcn]) ∧ (dependencies s.rtr i ⊆ s.progress) ∧ (i ∉ s.progress) where
@@ -104,11 +108,13 @@ theorem Triggers.congr {s₁ s₂ : State α}
 theorem Triggers.iff_record : s.Triggers i₂ ↔ (s.record i₁).Triggers i₂ :=
   Triggers.congr
 
+omit [Hierarchical α] in
 theorem NextTag.isLeast {s : State α} (n : NextTag s g) :
     IsLeast { g' ∈ s.scheduledTags | s.tag < g' } g where
   left := ⟨n.mem, n.bound⟩
   right := by simp [lowerBounds]; exact n.least
 
+omit [Hierarchical α] in
 theorem NextTag.deterministic {s : State α} (n₁ : NextTag s g₁) (n₂ : NextTag s g₂) : g₁ = g₂ :=
   n₁.isLeast.unique n₂.isLeast
 
@@ -138,7 +144,7 @@ theorem target_not_mem_indep_output
     (s.output i₁).Forall (¬·.Targets cpt i) := by
   apply List.forall_iff_forall_mem.mpr
   intro c hc
-  simp [output] at hc
+  simp only [output, Option.elim] at hc
   split at hc <;> try contradiction
   case _ rcn₁ h₁ =>
     cases cpt
