ReactorModel/Execution/Theorems/Step/Exec.lean
@@ -10,7 +10,7 @@ def rcn :                  (s₁ ↓ₑ s₂) → ID                            
 def applied :              (s₁ ↓ₑ s₂) → State α                          | mk (s₂ := s) .. => s
 theorem allows_rcn :   (e : s₁ ↓ₑ s₂) → Allows s₁ e.rcn                  | mk a .. => a
 theorem triggers_rcn : (e : s₁ ↓ₑ s₂) → Triggers s₁ e.rcn                | mk _ t _ => t
-theorem apply :        (e : s₁ ↓ₑ s₂) → s₁ -[s₁.output e.rcn]→ e.applied | mk _ _ a => a
+def apply :            (e : s₁ ↓ₑ s₂) → s₁ -[s₁.output e.rcn]→ e.applied | mk _ _ a => a
 theorem dst_eq :       (e : s₁ ↓ₑ s₂) → s₂ = e.applied.record e.rcn      | mk .. => rfl
 
 theorem applied_rtr_eq (e : s₁ ↓ₑ s₂) : e.applied.rtr = s₂.rtr := by
@@ -23,24 +23,24 @@ theorem preserves_tag (e : s₁ ↓ₑ s₂) : s₁.tag = s₂.tag := by
 theorem equiv (e : s₁ ↓ₑ s₂) : s₁.rtr ≈ s₂.rtr := by
   simp [e.dst_eq, State.record_preserves_rtr, e.apply.equiv]
 
-theorem progress_eq (e : s₁ ↓ₑ s₂) : s₂.progress = s₁.progress.insert e.rcn := by 
+theorem progress_eq (e : s₁ ↓ₑ s₂) : s₂.progress = s₁.progress.insert e.rcn := by
   simp [e.dst_eq, State.record_progress_eq, e.apply.preserves_progress]
 
 theorem preserves_nontrivial {e : s₁ ↓ₑ s₂} (n : s₁.Nontrivial) : s₂.Nontrivial :=
   n.equiv e.equiv
 
-theorem indep_allows_iff (e : s₁ ↓ₑ s₂) (hi : i ≮[s₁.rtr]≯ e.rcn) : 
+theorem indep_allows_iff (e : s₁ ↓ₑ s₂) (hi : i ≮[s₁.rtr]≯ e.rcn) :
     s₁.Allows i ↔ s₂.Allows i := by
   have a := e.apply
   simp [e.dst_eq, ←Allows.iff_record_indep (a.preserves_independent hi).symm, a.allows_iff]
-  
+
 theorem unprocessed_eq (e : s₁ ↓ₑ s₂) : s₂.unprocessed = s₁.unprocessed \ {e.rcn} := by
   ext i
   simp [State.unprocessed, Equivalent.obj?_rcn_eq e.equiv, and_assoc, e.progress_eq]
   intro _; simp [Set.insert]; push_neg; simp [and_comm]
 
-theorem rcn_mem_unprocessed (e : s₁ ↓ₑ s₂) : e.rcn ∈ s₁.unprocessed := 
-  ⟨e.allows_rcn.mem, e.allows_rcn.unprocessed⟩ 
+theorem rcn_mem_unprocessed (e : s₁ ↓ₑ s₂) : e.rcn ∈ s₁.unprocessed :=
+  ⟨e.allows_rcn.mem, e.allows_rcn.unprocessed⟩
 
 theorem unprocessed_ssubset (e : s₁ ↓ₑ s₂) : s₂.unprocessed ⊂ s₁.unprocessed := by
   simp [e.unprocessed_eq, Set.ssubset_iff_subset_ne]
@@ -52,36 +52,36 @@ namespace Execution.Step.Exec
 
 variable [Proper α] {s s₁ : State α} {rcn : Reaction}
 
-theorem indep_restriction_eq  
-    (e : s₁ ↓ₑ s₂) (hi : e.rcn ≮[s₁.rtr]≯ i) (ho : s₁.rtr[.rcn][i] = some rcn) : 
-    input.restriction s₁ rcn cpt = input.restriction s₂ rcn cpt := by 
+theorem indep_restriction_eq
+    (e : s₁ ↓ₑ s₂) (hi : e.rcn ≮[s₁.rtr]≯ i) (ho : s₁.rtr[.rcn][i] = some rcn) :
+    input.restriction s₁ rcn cpt = input.restriction s₂ rcn cpt := by
   simp [input.restriction]
-  apply Partial.ext_restrict 
+  apply Partial.ext_restrict
   intro _ hd
-  exact e.applied_rtr_eq ▸ e.apply.preserves_unchanged $ State.target_not_mem_indep_output ho hi hd  
+  exact e.applied_rtr_eq ▸ e.apply.preserves_unchanged $ State.target_not_mem_indep_output ho hi hd
 
-theorem indep_input_eq 
+theorem indep_input_eq
     (e : s₁ ↓ₑ s₂) (hi : e.rcn ≮[s₁.rtr]≯ i) (h₁ : s₁.rtr[.rcn][i] = some rcn)
-    (h₂ : s₂.rtr[.rcn][i] = some rcn) : s₁.input i = s₂.input i := by 
+    (h₂ : s₂.rtr[.rcn][i] = some rcn) : s₁.input i = s₂.input i := by
   simp [input, h₁, h₂]
   refine ⟨?_, e.preserves_tag⟩
   ext1
   exact e.indep_restriction_eq hi h₁
 
-theorem indep_output_eq (e : s₁ ↓ₑ s₂) (hi : e.rcn ≮[s₁.rtr]≯ i) : s₁.output i = s₂.output i := by 
+theorem indep_output_eq (e : s₁ ↓ₑ s₂) (hi : e.rcn ≮[s₁.rtr]≯ i) : s₁.output i = s₂.output i := by
   simp [output]
   have he := Equivalent.obj?_rcn_eq e.equiv
   cases h : s₁.rtr[.rcn][i] <;> simp [he ▸ h]
   simp [e.indep_input_eq hi h $ he ▸ h]
 
-theorem indep_comm 
-    (e₁ : s ↓ₑ s₁) (e₁₂ : s₁ ↓ₑ s₁₂) (e₂ : s ↓ₑ s₂) (e₂₁ : s₂ ↓ₑ s₂₁) 
-    (hr₁ : e₁.rcn = e₂₁.rcn) (hr₂ : e₂.rcn = e₁₂.rcn) (hi : e₁.rcn ≮[s.rtr]≯ e₂.rcn) : 
-    s₁₂ = s₂₁ := by 
+theorem indep_comm
+    (e₁ : s ↓ₑ s₁) (e₁₂ : s₁ ↓ₑ s₁₂) (e₂ : s ↓ₑ s₂) (e₂₁ : s₂ ↓ₑ s₂₁)
+    (hr₁ : e₁.rcn = e₂₁.rcn) (hr₂ : e₂.rcn = e₁₂.rcn) (hi : e₁.rcn ≮[s.rtr]≯ e₂.rcn) :
+    s₁₂ = s₂₁ := by
   have ho₁ := e₁.indep_output_eq hi
   have ho₂ := e₂.indep_output_eq hi.symm
   cases e₁; cases e₁₂; cases e₂; cases e₂₁
-  case _ rcn₁ s₁ _ _ a₁ rcn₂ s₁₂ _ _ a₁₂ _ s₂ _ _ a₂ _ s₂₁ _ _ a₂₁ => 
+  case _ rcn₁ s₁ _ _ a₁ rcn₂ s₁₂ _ _ a₁₂ _ s₂ _ _ a₂ _ s₂₁ _ _ a₂₁ =>
     cases hr₁; cases hr₂; simp [Exec.rcn] at *
     have ⟨z₁₂, f₁₂⟩ := Apply.RTC.construct s₁ (s.output rcn₂)
     have ⟨z₂₁, f₂₁⟩ := Apply.RTC.construct s₂ (s.output rcn₁)
@@ -90,16 +90,16 @@ theorem indep_comm
     rw [record_comm]; congr
     exact Apply.RTC.disjoint_targets_comm (s.indep_output_disjoint_targets hi) a₁ f₁₂ a₂ f₂₁
 
-theorem indep_triggers_iff (e : s₁ ↓ₑ s₂) (hi : i ≮[s₁.rtr]≯ e.rcn) : 
+theorem indep_triggers_iff (e : s₁ ↓ₑ s₂) (hi : i ≮[s₁.rtr]≯ e.rcn) :
     s₁.Triggers i ↔ s₂.Triggers i := by
-  constructor <;> intro ⟨ho, ht⟩  
+  constructor <;> intro ⟨ho, ht⟩
   case mp =>
     have ho' := Equivalent.obj?_rcn_eq e.equiv ▸ ho
     have ht' := e.indep_input_eq hi.symm ‹_› ‹_› ▸ ht
-    exact ⟨ho', ht'⟩ 
+    exact ⟨ho', ht'⟩
   case mpr =>
     have ho' := Equivalent.obj?_rcn_eq e.equiv |>.symm ▸ ho
     have ht' := e.indep_input_eq hi.symm ‹_› ‹_› |>.symm ▸ ht
-    exact ⟨ho', ht'⟩ 
+    exact ⟨ho', ht'⟩
 
 end Execution.Step.Exec
