ReactorModel/Objects/Reactor/Theorems/Basic.lean
@@ -28,11 +28,11 @@ instance : Equivalence ((· : α) ≃[cpt][i] ·) :=
 
 theorem mem_iff (e : rtr₁ ≃[cpt][i] rtr₂) (h : c ≠ cpt ∨ j ≠ i) : j ∈ rtr₁{c} ↔ j ∈ rtr₂{c} := by
   simp [Partial.mem_iff]
-  exact ⟨(e h ▸ ·), (e h ▸ ·)⟩   
+  exact ⟨(e h ▸ ·), (e h ▸ ·)⟩
 
-theorem valued {c cpt : Component.Valued} (e : rtr₁ ≃[cpt][i] rtr₂) (h : c ≠ cpt ∨ j ≠ i) : 
-    rtr₁{c}{j} = rtr₂{c}{j} := 
-  e $ h.elim (by simp [*]) Or.inr  
+theorem valued {c cpt : Component.Valued} (e : rtr₁ ≃[cpt][i] rtr₂) (h : c ≠ cpt ∨ j ≠ i) :
+    rtr₁{c}{j} = rtr₂{c}{j} :=
+  e $ h.elim (by simp [*]) Or.inr
 
 end RootEqualUpTo
 
@@ -41,23 +41,23 @@ end RootEqualUpTo
 inductive Equivalent [inst : Reactor α] : α → α → Prop
   | refl (rtr) : Equivalent rtr rtr
   | struct
-    (mem_get?_iff : ∀ cpt i, i ∈ rtr₁{cpt} ↔ i ∈ rtr₂{cpt}) 
-    (get?_rcn_some_eq : ∀ {i r₁ r₂}, (rtr₁{.rcn}{i} = some r₁) → (rtr₂{.rcn}{i} = some r₂) → r₁ = r₂) 
-    (get?_rtr_some_equiv : ∀ {i n₁ n₂}, (rtr₁{.rtr}{i} = some n₁) → (rtr₂{.rtr}{i} = some n₂) → Equivalent (inst := inst) n₁ n₂) 
+    (mem_get?_iff : ∀ cpt i, i ∈ rtr₁{cpt} ↔ i ∈ rtr₂{cpt})
+    (get?_rcn_some_eq : ∀ {i r₁ r₂}, (rtr₁{.rcn}{i} = some r₁) → (rtr₂{.rcn}{i} = some r₂) → r₁ = r₂)
+    (get?_rtr_some_equiv : ∀ {i n₁ n₂}, (rtr₁{.rtr}{i} = some n₁) → (rtr₂{.rtr}{i} = some n₂) → Equivalent (inst := inst) n₁ n₂)
     : Equivalent rtr₁ rtr₂
- 
+
 namespace Equivalent
 
 variable [Reactor α] {rtr₁ : α}
 
-instance : HasEquiv α where 
+instance : HasEquiv α where
   Equiv := Equivalent
 
 @[symm]
 theorem symm (e : rtr₁ ≈ rtr₂) : rtr₂ ≈ rtr₁ := by
   induction e
   case refl => exact .refl _
-  case struct h₁ h₂ _ hi => 
+  case struct h₁ h₂ _ hi =>
     constructor <;> intros
     · exact h₁ ‹_› ‹_› |>.symm
     · exact h₂ ‹_› ‹_› |>.symm
@@ -69,35 +69,35 @@ theorem trans (e₁ : rtr₁ ≈ rtr₂) (e₂ : rtr₂ ≈ rtr₃) : rtr₁ ≈
   case refl => exact e₂
   case struct h₁ h₂ _ hi =>
     cases e₂
-    case refl => exact .struct ‹_› ‹_› ‹_› 
-    case struct h₁' h₂' h₃'=> 
+    case refl => exact .struct ‹_› ‹_› ‹_›
+    case struct h₁' h₂' h₃'=>
       apply Equivalent.struct
       · intros; exact h₁ ‹_› ‹_› |>.trans (h₁' ‹_› ‹_›)
       · intro _ _ _ h _
         have ⟨_, h⟩ := Partial.mem_iff.mp <| h₁ .rcn ‹_› |>.mp $ Partial.mem_iff.mpr ⟨_, h⟩
         exact h₂ ‹_› h |>.trans (h₂' h ‹_›)
       · intro _ _ _ h _
-        have ⟨_, h⟩ := Partial.mem_iff.mp <| h₁ .rtr ‹_› |>.mp $ Partial.mem_iff.mpr ⟨_, h⟩ 
+        have ⟨_, h⟩ := Partial.mem_iff.mp <| h₁ .rtr ‹_› |>.mp $ Partial.mem_iff.mpr ⟨_, h⟩
         exact hi ‹_› h (h₃' h ‹_›)
 
-instance : Equivalence ((· : α) ≈ ·) := 
+instance : Equivalence ((· : α) ≈ ·) :=
   { refl, symm, trans }
 
 theorem mem_get?_iff : (rtr₁ ≈ rtr₂) → (i ∈ rtr₁{cpt} ↔ i ∈ rtr₂{cpt})
   | refl _      => Iff.refl _
   | struct h .. => h _ _
 
-theorem get?_rcn_some_eq : 
+theorem get?_rcn_some_eq :
     (rtr₁ ≈ rtr₂) → (rtr₁{.rcn}{i} = some r₁) → (rtr₂{.rcn}{i} = some r₂) → r₁ = r₂
   | refl _       => by simp_all
   | struct _ h _ => h
 
-theorem get?_rtr_some_equiv : 
+theorem get?_rtr_some_equiv :
     (rtr₁ ≈ rtr₂) → (rtr₁{.rtr}{i} = some n₁) → (rtr₂{.rtr}{i} = some n₂) → n₁ ≈ n₂
   | refl _       => by intros; simp_all; exact .refl _
   | struct _ _ h => h
 
-theorem get?_some_iff (e : rtr₁ ≈ rtr₂) : 
+theorem get?_some_iff (e : rtr₁ ≈ rtr₂) :
     (∃ o, rtr₁{cpt}{i} = some o) ↔ (∃ o, rtr₂{cpt}{i} = some o) := by
   simp [←Partial.mem_iff, mem_get?_iff e]
 
@@ -131,7 +131,7 @@ def member₁ {rtr₁ : α} : (LawfulMemUpdate cpt i v rtr₁ rtr₂) → Strict
 def member₂ {rtr₁ : α} : (LawfulMemUpdate cpt i v rtr₁ rtr₂) → StrictMember cpt i rtr₂
   | final _ _ h  => .final h
   | nested _ _ h u => .nested h u.member₂
-  
+
 theorem equiv {rtr₁ : α} (u : LawfulMemUpdate cpt i v rtr₁ rtr₂) : rtr₁ ≈ rtr₂ := by
   induction u <;> constructor
   case final.mem_get?_iff e h₁ h₂ =>
@@ -155,7 +155,7 @@ theorem equiv {rtr₁ : α} (u : LawfulMemUpdate cpt i v rtr₁ rtr₂) : rtr₁
     intro c j'
     by_cases hc : c = .rtr <;> try subst hc
     case neg => exact e.mem_iff (.inl hc)
-    case pos => 
+    case pos =>
       by_cases hj : j' = j <;> try subst hj
       case neg => exact e.mem_iff (.inr hj)
       case pos => simp [Partial.mem_iff, h₁, h₂]
@@ -167,7 +167,7 @@ theorem equiv {rtr₁ : α} (u : LawfulMemUpdate cpt i v rtr₁ rtr₂) : rtr₁
     intro j' n₁' n₂' h₁' h₂'
     by_cases hj : j' = j <;> try subst hj
     case pos => simp_all; assumption
-    case neg => 
+    case neg =>
       have := e (c := .rtr) (j := j') (.inr hj)
       simp_all
       apply Equivalent.refl
@@ -179,8 +179,8 @@ theorem LawfulUpdate.equiv [Reactor α] {rtr₁ : α} :
   | notMem _ h => h ▸ (.refl _)
   | update u   => u.equiv
 
-theorem LawfulUpdatable.equiv [LawfulUpdatable α] {rtr : α} : 
-    rtr ≈ (Updatable.update rtr cpt i f) := 
+theorem LawfulUpdatable.equiv [LawfulUpdatable α] {rtr : α} :
+    rtr ≈ (Updatable.update rtr cpt i f) :=
   (lawful rtr cpt i f).equiv
 
 /- ---------------------------------------------------------------------------------------------- -/
@@ -189,28 +189,28 @@ namespace StrictMember
 variable [Reactor α] {rtr : α} in section
 
 theorem nested_object (s : StrictMember cpt i' rtr') (h : rtr{.rtr}{i} = some rtr') :
-    (nested h s).object = s.object := 
+    (nested h s).object = s.object :=
   rfl
 
-def split : 
-    {rtr rtr' : α} → (s : StrictMember cpt i' rtr') → (rtr{.rtr}{i} = some rtr') → 
+def split :
+    {rtr rtr' : α} → (s : StrictMember cpt i' rtr') → (rtr{.rtr}{i} = some rtr') →
     (j : ID) × { s' : StrictMember .rtr j rtr // s'.object{cpt}{i'} = s.object }
   | _, _, final hn, h => ⟨i, ⟨final h, hn⟩⟩
   | _, _, nested hn s, h => let ⟨j, ⟨s', hs'⟩⟩ := split s hn; ⟨j, ⟨nested h s', hs'⟩⟩
 
-def split' : 
-    (s : StrictMember cpt i rtr) → 
-    (j : WithTop ID) × { m : Member .rtr j rtr // m.object{cpt}{i} = s.object } 
+def split' :
+    (s : StrictMember cpt i rtr) →
+    (j : WithTop ID) × { m : Member .rtr j rtr // m.object{cpt}{i} = s.object }
   | final h     => ⟨⊤, ⟨.root, h⟩⟩
   | nested hn s => let ⟨j, ⟨s', hs'⟩⟩ := split s hn; ⟨j, ⟨.strict s', hs'⟩⟩
 
-def extend : 
+def extend :
     {rtr : α} → (s : StrictMember .rtr i rtr) → (s.object{cpt}{j} = some o) → StrictMember cpt j rtr
   | _, final hn,    h => nested hn (final h)
   | _, nested hn s, h => nested hn (extend s h)
 
 theorem extend_object :
-    {rtr : α} → (s : StrictMember .rtr i rtr) → (h : s.object{cpt}{j} = some o) → 
+    {rtr : α} → (s : StrictMember .rtr i rtr) → (h : s.object{cpt}{j} = some o) →
     (s.extend h).object = o
   | _, final _,    _ => rfl
   | _, nested _ s, h => extend_object s h
@@ -219,12 +219,12 @@ theorem extend_not_final (s : StrictMember .rtr i rtr) (h : s.object{cpt}{j} = s
     (hf : rtr{cpt}{j} = some o') : s.extend h ≠ final hf := by
   cases s <;> simp [extend]
 
-theorem extend_inj 
+theorem extend_inj
     {s₁ : StrictMember .rtr i₁ rtr} {s₂ : StrictMember .rtr i₂ rtr}
     {h₁ : s₁.object{cpt}{j} = some o₁} {h₂ : s₂.object{cpt}{j} = some o₂}
     (h : s₁.extend h₁ = s₂.extend h₂) : i₁ = i₂ := by
   induction s₁ generalizing i₂ <;> cases s₂
-  all_goals simp [extend] at h; obtain ⟨hj, hr, h⟩ := h; subst hj hr 
+  all_goals simp [extend] at h; obtain ⟨hj, hr, h⟩ := h; subst hj hr
   case final.final  => rfl
   case nested.nested hi _ _ => exact hi $ eq_of_heq h
   case final.nested => exact absurd (eq_of_heq h).symm $ StrictMember.extend_not_final _ _ _
@@ -235,49 +235,49 @@ theorem extend_split (s : StrictMember cpt i' rtr') (h : rtr{.rtr}{i} = some rtr
   induction s generalizing rtr i <;> simp [extend]
   case nested h' _ hi => exact hi h'
 
-def fromLawfulMemUpdate {rtr₁ : α} : 
+def fromLawfulMemUpdate {rtr₁ : α} :
     (StrictMember c j rtr₂) → (LawfulMemUpdate cpt i v rtr₁ rtr₂) → StrictMember c j rtr₁
   | final h, u               => final $ (Equivalent.get?_some_iff u.equiv).mpr ⟨_, h⟩ |>.choose_spec
-  | nested h s, .final e _ _ => nested (h ▸ e (.inl $ by simp)) s 
+  | nested h s, .final e _ _ => nested (h ▸ e (.inl $ by simp)) s
   | nested h s (j := j₂), .nested e h₁ h₂ u (j := j₁) =>
-      if hj : j₂ = j₁ 
+      if hj : j₂ = j₁
       then nested h₁ $ fromLawfulMemUpdate ((Option.some_inj.mp $ h₂ ▸ hj ▸ h) ▸ s) u
-      else nested (h ▸ e $ .inr hj) s 
+      else nested (h ▸ e $ .inr hj) s
 
-def fromLawfulUpdate {rtr₂ : α} (s : StrictMember c j rtr₂) : 
+def fromLawfulUpdate {rtr₂ : α} (s : StrictMember c j rtr₂) :
     (LawfulUpdate cpt i v rtr₁ rtr₂) → StrictMember c j rtr₁
   | .notMem _ h => h ▸ s
   | .update u   => s.fromLawfulMemUpdate u
 
-def fromEquiv {rtr₁ : α} (e : rtr₁ ≈ rtr₂) : 
+def fromEquiv {rtr₁ : α} (e : rtr₁ ≈ rtr₂) :
     (StrictMember cpt i rtr₁) → StrictMember cpt i rtr₂
   | final h    => final (e.get?_some_iff.mp ⟨_, h⟩).choose_spec
-  | nested h m => 
-    have h' := (Equivalent.get?_some_iff e).mp ⟨_, h⟩ 
+  | nested h m =>
+    have h' := (Equivalent.get?_some_iff e).mp ⟨_, h⟩
     have e' := Equivalent.get?_rtr_some_equiv e h h'.choose_spec
     nested h'.choose_spec (fromEquiv e' m)
 
 end
 
-inductive Equivalent : 
-    {α : Type} → {β : Type} → [Reactor α] → [Reactor β] → {rtr₁ : α} → {rtr₂ : β} → 
-    (StrictMember cpt i rtr₁) → (StrictMember cpt i rtr₂) → Prop 
+inductive Equivalent :
+    {α : Type} → {β : Type} → [Reactor α] → [Reactor β] → {rtr₁ : α} → {rtr₂ : β} →
+    (StrictMember cpt i rtr₁) → (StrictMember cpt i rtr₂) → Prop
   | refl [Reactor α] {rtr : α} (s : StrictMember cpt i rtr) : Equivalent s s
-  | final [Reactor α] [Reactor β] {rtr₁ : α} {rtr₂ : β} 
+  | final [Reactor α] [Reactor β] {rtr₁ : α} {rtr₂ : β}
     (h₁ : rtr₁{cpt}{i} = some o₁) (h₂ : rtr₂{cpt}{i} = some o₂) : Equivalent (final h₁) (final h₂)
-  | nested [Reactor α] [Reactor β] {rtr₁ : α} {rtr₂ : β} {n₁ : α} {n₂ : β} 
-    {s₁ : StrictMember cpt i n₁} {s₂ : StrictMember cpt i n₂} (h₁ : rtr₁{.rtr}{j} = some n₁) 
+  | nested [Reactor α] [Reactor β] {rtr₁ : α} {rtr₂ : β} {n₁ : α} {n₂ : β}
+    {s₁ : StrictMember cpt i n₁} {s₂ : StrictMember cpt i n₂} (h₁ : rtr₁{.rtr}{j} = some n₁)
     (h₂ : rtr₂{.rtr}{j} = some n₂) : (Equivalent s₁ s₂) → Equivalent (nested h₁ s₁) (nested h₂ s₂)
 
 namespace Equivalent
 
 variable [Reactor α] {rtr₁ : α}
 
-instance [Reactor β] {rtr₂ : β} : 
+instance [Reactor β] {rtr₂ : β} :
     HasHEquiv (StrictMember cpt i rtr₁) (StrictMember cpt i rtr₂) where
   HEquiv := Equivalent (cpt := cpt) (i := i) (rtr₁ := rtr₁) (rtr₂ := rtr₂)
 
-theorem symm [Reactor β] {rtr₂ : β} 
+theorem symm [Reactor β] {rtr₂ : β}
     {s₁ : StrictMember cpt i rtr₁} {s₂ : StrictMember cpt i rtr₂} (e : s₁ ∼ s₂) : s₂ ∼ s₁ := by
   induction e <;> constructor; assumption
 
@@ -287,7 +287,7 @@ theorem trans [Reactor β] [Reactor γ] {rtr₂ : β} {rtr₃ : γ}
   induction e₁ generalizing rtr₃ <;> cases e₂ <;> constructor <;> try assumption
   case nested.nested hi₁ _ _ _ _ hi₂ => exact hi₁ hi₂
 
-instance {rtr : α} : Equivalence (Equivalent (· : StrictMember cpt i rtr) ·) := 
+instance {rtr : α} : Equivalence (Equivalent (· : StrictMember cpt i rtr) ·) :=
   { refl, symm, trans }
 
 theorem to_eq {rtr : α} {s₁ s₂ : StrictMember cpt i rtr} : (s₁ ∼ s₂) → s₁ = s₂
@@ -295,20 +295,20 @@ theorem to_eq {rtr : α} {s₁ s₂ : StrictMember cpt i rtr} : (s₁ ∼ s₂) 
   | final h₁ h₂    => by simp [Option.some_inj.mp $ h₁ ▸ h₂]
   | nested h₁ h₂ e => by cases Option.some_inj.mp $ h₁ ▸ h₂; simp [to_eq e]
 
-theorem fromLawfulMemUpdate (u : LawfulMemUpdate cpt i v rtr₁ rtr₂) (s : StrictMember c j rtr₂) : 
+theorem fromLawfulMemUpdate (u : LawfulMemUpdate cpt i v rtr₁ rtr₂) (s : StrictMember c j rtr₂) :
     s ∼ s.fromLawfulMemUpdate u := by
   induction u <;> cases s <;> (simp [StrictMember.fromLawfulMemUpdate]; try exact final _ _)
   case final.nested e _ _ _ _ _ hn => exact nested hn (e (c := .rtr) (.inl $ by simp) ▸ hn) (refl _)
   case nested.nested e h₁ h₂ _ hi _ _ m hn =>
     split
-    case inl hj => cases hj; cases Option.some_inj.mp $ h₂ ▸ hn; exact nested hn h₁ (hi m)
-    case inr hj => exact nested hn (hn ▸ e (.inr hj)) (refl _)
+    case isTrue  hj => cases hj; cases Option.some_inj.mp $ h₂ ▸ hn; exact nested hn h₁ (hi m)
+    case isFalse hj => exact nested hn (hn ▸ e (.inr hj)) (refl _)
 
-theorem fromLawfulUpdate (u : LawfulUpdate cpt i v rtr₁ rtr₂) (s : StrictMember c j rtr₂) : 
+theorem fromLawfulUpdate (u : LawfulUpdate cpt i v rtr₁ rtr₂) (s : StrictMember c j rtr₂) :
     s ∼ s.fromLawfulUpdate u := by
   cases u
   case notMem   => cases ‹_ = _›; apply refl
-  case update u => exact fromLawfulMemUpdate u s 
+  case update u => exact fromLawfulMemUpdate u s
 
 end Equivalent
 end StrictMember
@@ -322,13 +322,13 @@ def extend : (m : Member .rtr i rtr) → (m.object{cpt}{j} = some o) → Member 
   | root,     h => final h
   | strict s, h => s.extend h
 
-theorem extend_object : 
+theorem extend_object :
     (m : Member .rtr i rtr) → (h : m.object{cpt}{j} = some o) → (m.extend h).object = o
   | root,     h => rfl
   | strict s, h => s.extend_object h
 
 theorem extend_inj
-    {m₁ : Member .rtr i₁ rtr} {m₂ : Member .rtr i₂ rtr} {h₁ : m₁.object{cpt}{j} = some o₁} 
+    {m₁ : Member .rtr i₁ rtr} {m₂ : Member .rtr i₂ rtr} {h₁ : m₁.object{cpt}{j} = some o₁}
     {h₂ : m₂.object{cpt}{j} = some o₂} (h : m₁.extend h₁ = m₂.extend h₂) : i₁ = i₂ := by
   cases m₁ <;> cases m₂ <;> simp [Member.extend] at h
   case root.root     => rfl
@@ -336,10 +336,10 @@ theorem extend_inj
   case root.strict   => exact absurd h.symm $ StrictMember.extend_not_final _ _ _
   case strict.root   => exact absurd h $ StrictMember.extend_not_final _ _ _
 
-def fromLawfulMemUpdate (m : Member c j rtr₂) (u : LawfulMemUpdate cpt i v rtr₁ rtr₂) : 
+def fromLawfulMemUpdate (m : Member c j rtr₂) (u : LawfulMemUpdate cpt i v rtr₁ rtr₂) :
     Member c j rtr₁ :=
   match m with
-  | root => root 
+  | root => root
   | strict s => s.fromLawfulMemUpdate u
 
 def fromLawfulUpdate (m : Member c j rtr₂) (u : LawfulUpdate cpt i v rtr₁ rtr₂) : Member c j rtr₁ :=
@@ -351,7 +351,7 @@ def fromEquiv (e : rtr₁ ≈ rtr₂) : (Member cpt i rtr₁) → Member cpt i r
   | root     => root
   | strict s => s.fromEquiv e
 
-inductive Equivalent [Reactor β] {rtr₂ : β} : (Member cpt i rtr₁) → (Member cpt i rtr₂) → Prop 
+inductive Equivalent [Reactor β] {rtr₂ : β} : (Member cpt i rtr₁) → (Member cpt i rtr₂) → Prop
   | root   : Equivalent root root
   | strict : (StrictMember.Equivalent s₁ s₂) → Equivalent (strict s₁) (strict s₂)
 
@@ -364,11 +364,11 @@ theorem refl : (m : Member cpt i rtr) → m ∼ m
   | .root     => root
   | .strict s => strict $ .refl s
 
-theorem symm [Reactor β] {rtr₂ : β} {m₁ : Member cpt i rtr₁} {m₂ : Member cpt i rtr₂} 
+theorem symm [Reactor β] {rtr₂ : β} {m₁ : Member cpt i rtr₁} {m₂ : Member cpt i rtr₂}
     (e : m₁ ∼ m₂) : m₂ ∼ m₁ := by
-  cases m₁ 
+  cases m₁
   case root => cases m₂; exact root
-  case strict => cases cpt <;> cases e <;> exact .strict $ StrictMember.Equivalent.symm ‹_›  
+  case strict => cases cpt <;> cases e <;> exact .strict $ StrictMember.Equivalent.symm ‹_›
 
 theorem trans [Reactor β] [Reactor γ] {rtr₂ : β} {rtr₃ : γ}
     {m₁ : Member cpt i rtr₁} {m₂ : Member cpt i rtr₂} {m₃ : Member cpt i rtr₃}
@@ -376,24 +376,24 @@ theorem trans [Reactor β] [Reactor γ] {rtr₂ : β} {rtr₃ : γ}
   cases m₁
   case root => cases m₃; exact root
   case strict =>
-    cases cpt <;> cases e₁ <;> cases e₂ <;> exact .strict $ StrictMember.Equivalent.trans ‹_› ‹_›  
+    cases cpt <;> cases e₁ <;> cases e₂ <;> exact .strict $ StrictMember.Equivalent.trans ‹_› ‹_›
 
-instance : Equivalence (Equivalent (· : Member cpt i rtr) ·) := 
+instance : Equivalence (Equivalent (· : Member cpt i rtr) ·) :=
   { refl, symm, trans }
 
 theorem to_eq {m₁ m₂ : Member cpt i rtr} : (m₁ ∼ m₂) → m₁ = m₂
   | root     => rfl
   | strict e => congr_arg _ $ StrictMember.Equivalent.to_eq e
 
-theorem fromLawfulMemUpdate (u : LawfulMemUpdate cpt i v rtr₁ rtr₂) : 
+theorem fromLawfulMemUpdate (u : LawfulMemUpdate cpt i v rtr₁ rtr₂) :
     (m : Member c j rtr₂) → m ∼ m.fromLawfulMemUpdate u
   | .root     => root
-  | .strict s => strict $ .fromLawfulMemUpdate u s 
+  | .strict s => strict $ .fromLawfulMemUpdate u s
 
 theorem fromLawfulUpdate (u : LawfulUpdate cpt i v rtr₁ rtr₂) :
     (m : Member c j rtr₂) → m ∼ m.fromLawfulUpdate u
   | .root     => root
-  | .strict s => strict $ .fromLawfulUpdate u s 
+  | .strict s => strict $ .fromLawfulUpdate u s
 
 end Equivalent
 end Member
@@ -404,8 +404,8 @@ namespace Object
 variable [Reactor α] {rtr rtr₁ : α}
 
 theorem «def» : (Object rtr cpt i o) ↔ (∃ m : Member cpt i rtr, m.object = o) where
-  mp  | ⟨m⟩    => ⟨m, rfl⟩ 
-  mpr | ⟨m, h⟩ => h ▸ ⟨m⟩   
+  mp  | ⟨m⟩    => ⟨m, rfl⟩
+  mpr | ⟨m, h⟩ => h ▸ ⟨m⟩
 
 theorem strict_elim {i : ID} : (Object rtr cpt i o) → ∃ (s : StrictMember cpt i rtr), s.object = o
   | ⟨m⟩ => by cases cpt <;> cases m <;> exists ‹_›
@@ -417,7 +417,7 @@ theorem equiv_exists_object_iff (e : rtr₁ ≈ rtr₂) :
     (∃ o₁, Object rtr₁ cpt i o₁) ↔ (∃ o₂, Object rtr₂ cpt i o₂) where
   mp  | ⟨_, ⟨m⟩⟩ => ⟨_, ⟨m.fromEquiv e⟩⟩
   mpr | ⟨_, ⟨m⟩⟩ => ⟨_, ⟨m.fromEquiv $ Equivalent.symm e⟩⟩
-  
+
 end Object
 
 /- ---------------------------------------------------------------------------------------------- -/
@@ -427,7 +427,7 @@ variable [Reactor α] {rtr₁ : α}
 
 theorem updated (u : LawfulUpdate cpt i v rtr₁ rtr₂) (h : UniqueIDs rtr₁) : UniqueIDs rtr₂ where
   allEq m₁ m₂ := open Member.Equivalent in
-    to_eq $ trans 
+    to_eq $ .trans
       (h.allEq (m₁.fromLawfulUpdate u) (m₂.fromLawfulUpdate u) ▸ fromLawfulUpdate u m₁)
       (symm (fromLawfulUpdate u m₂))
 
