ReactorModel/Objects/Reactor/Theorems/Hierarchical.lean
@@ -11,34 +11,36 @@ variable [Hierarchical α] {rtr rtr₁ : α}
 theorem unique (s₁ s₂ : StrictMember cpt i rtr) : s₁ = s₂ := by
   injection unique_ids.allEq (.strict s₁) (.strict s₂)
 
-theorem equiv 
+theorem equiv
     (e : rtr₁ ≈ rtr₂) (s₁ : StrictMember cpt i rtr₁) (s₂ : StrictMember cpt i rtr₂) : s₁ ∼ s₂ := by
   induction s₁ generalizing rtr₂ <;> cases s₂
   case final.final => constructor
   case nested.nested rtr₁ j₁ _ h₁ s₁ hi j₂ _ s₂ h₂ =>
-    suffices hj : j₁ = j₂ by 
+    suffices hj : j₁ = j₂ by
       subst hj
       exact Equivalent.nested h₁ h₂ $ hi (Equivalent.get?_rtr_some_equiv e h₁ h₂) s₂
     have hs := (nested h₁ s₁ |>.fromEquiv e).unique (nested h₂ s₂)
     simp [fromEquiv] at hs
     exact hs.left
-  case final.nested h₁ _ _ s₂ h₂ => 
-    injection (final h₁ |>.fromEquiv e).unique (nested h₂ s₂)
+  case final.nested h₁ _ _ s₂ h₂ =>
+    have h := (final h₁ |>.fromEquiv e).unique (nested h₂ s₂)
+    simp [fromEquiv] at h
   case nested.final h₁ s₁ _ _ h₂ =>
-    injection (nested h₁ s₁).unique (final h₂ |>.fromEquiv $ Reactor.Equivalent.symm e) 
+    have h := (nested h₁ s₁).unique (final h₂ |>.fromEquiv $ Reactor.Equivalent.symm e)
+    simp [fromEquiv] at h
 
--- TODO: In all three of the following theorems, the `final.nested` and `nested.final` cases could 
+-- TODO: In all three of the following theorems, the `final.nested` and `nested.final` cases could
 --       be removed if we figure out how to use the above `equiv` theorem. Induction on the
---       membership witness equivalence doesn't seem to work. Perhaps you need to prove a custom 
+--       membership witness equivalence doesn't seem to work. Perhaps you need to prove a custom
 --       induction principle for `StrictMember.Equivalent`. This would also remove the need to prove
---       things like `j₁ = j₂` in the `nested` case each time. 
+--       things like `j₁ = j₂` in the `nested` case each time.
 --
 --       Note that both of the following theorems are almost identical. The only difference happens
 --       in the "local" view of things in the `final.final` case. Perhaps there's a more general
 --       theorem here for lifting local properties to global properties. Though since these
 --       properties are tied to `Equivalent`, it might not be generalizable.
 
-theorem rtr_equiv 
+theorem rtr_equiv
     (e : rtr₁ ≈ rtr₂) (s₁ : StrictMember .rtr i rtr₁) (s₂ : StrictMember .rtr i rtr₂) :
     s₁.object ≈ s₂.object := by
   induction s₁ generalizing rtr₂ <;> cases s₂
@@ -48,27 +50,31 @@ theorem rtr_equiv
     have hs := (nested h₁ s₁ |>.fromEquiv e).unique (nested h₂ s₂)
     simp [fromEquiv] at hs
     exact hs.left
-  case final.nested h₁ _ _ s₂ h₂ => 
-    injection (final h₁ |>.fromEquiv e).unique (nested h₂ s₂)
+  case final.nested h₁ _ _ s₂ h₂ =>
+    have h := (final h₁ |>.fromEquiv e).unique (nested h₂ s₂)
+    simp [fromEquiv] at h
   case nested.final h₁ s₁ _ _ h₂ =>
-    injection (nested h₁ s₁).unique (final h₂ |>.fromEquiv $ Reactor.Equivalent.symm e) 
+    have h := (nested h₁ s₁).unique (final h₂ |>.fromEquiv $ Reactor.Equivalent.symm e)
+    simp [fromEquiv] at h
 
-theorem equiv_rcn_eq 
-    (e : rtr₁ ≈ rtr₂) (s₁ : StrictMember .rcn i rtr₁) (s₂ : StrictMember .rcn i rtr₂) : 
+theorem equiv_rcn_eq
+    (e : rtr₁ ≈ rtr₂) (s₁ : StrictMember .rcn i rtr₁) (s₂ : StrictMember .rcn i rtr₂) :
     s₁.object = s₂.object := by
-  induction s₁ generalizing rtr₂ <;> cases s₂ 
+  induction s₁ generalizing rtr₂ <;> cases s₂
   case final.final h₁ _ h₂ => exact Equivalent.get?_rcn_some_eq e h₁ h₂
-  case nested.nested j₁ _ h₁ s₁ hi j₂ _ s₂ h₂ => 
-    suffices hj : j₁ = j₂ by subst hj; exact hi (Equivalent.get?_rtr_some_equiv e h₁ h₂) _ 
+  case nested.nested j₁ _ h₁ s₁ hi j₂ _ s₂ h₂ =>
+    suffices hj : j₁ = j₂ by subst hj; exact hi (Equivalent.get?_rtr_some_equiv e h₁ h₂) _
     have hs := (nested h₁ s₁ |>.fromEquiv e).unique (nested h₂ s₂)
     simp [fromEquiv] at hs
     exact hs.left
   case final.nested h₁ _ _ s₂ h₂ =>
-    injection (final h₁ |>.fromEquiv e).unique (nested h₂ s₂)
+    have h := (final h₁ |>.fromEquiv e).unique (nested h₂ s₂)
+    simp [fromEquiv] at h
   case nested.final h₁ s₁ _ _ h₂ =>
-    injection (nested h₁ s₁).unique (final h₂ |>.fromEquiv $ Reactor.Equivalent.symm e) 
+    have h := (nested h₁ s₁).unique (final h₂ |>.fromEquiv $ Reactor.Equivalent.symm e)
+    simp [fromEquiv] at h
 
-theorem lawfulMemUpdate_object_preserved 
+theorem lawfulMemUpdate_object_preserved
     (u : LawfulMemUpdate cpt i v rtr₁ rtr₂) (h : c ≠ cpt ∨ j ≠ i) (s₁ : StrictMember c j rtr₁)
     (s₂ : StrictMember c j rtr₂) : s₁.object = s₂.object := by
   induction s₁ generalizing rtr₂ <;> cases s₂ <;> simp [object]
@@ -76,28 +82,30 @@ theorem lawfulMemUpdate_object_preserved
     cases u
     case final e => simp_all [e.valued h]
     case nested e => simp_all [e (c := c) (.inl $ by simp)]
-  case nested.nested j₁ _ h₁ s₁ hi j₂ _ s₂ h₂ => 
-    have hj : j₁ = j₂ := by 
+  case nested.nested j₁ _ h₁ s₁ hi j₂ _ s₂ h₂ =>
+    have hj : j₁ = j₂ := by
       have hs := (nested h₁ s₁ |>.fromEquiv u.equiv).unique (nested h₂ s₂)
       simp [fromEquiv] at hs
       exact hs.left
     subst hj
     cases u
-    case final e => 
+    case final e =>
       cases h₂ ▸ (e (c := .rtr) (j := j₁) (.inl $ by simp)) ▸ h₁
       simp [s₁.unique s₂]
     case nested j' _ _ u _ _ e =>
       by_cases hj : j₁ = j'
-      case neg => 
+      case neg =>
         cases h₂ ▸ (e (c := .rtr) (j := j₁) (.inr hj)) ▸ h₁
         simp [s₁.unique s₂]
-      case pos => 
+      case pos =>
         simp_all [hj]
         exact hi (h₁ ▸ h₂ ▸ u) _
   case final.nested h₁ _ _ s₂ h₂ =>
-    injection (final h₁ |>.fromEquiv u.equiv).unique (nested h₂ s₂)
+    have h := (final h₁ |>.fromEquiv u.equiv).unique (nested h₂ s₂)
+    simp [fromEquiv] at h
   case nested.final h₁ s₁ _ _ h₂ =>
-    injection (nested h₁ s₁).unique (final h₂ |>.fromEquiv $ Reactor.Equivalent.symm u.equiv)     
+    have h := (nested h₁ s₁).unique (final h₂ |>.fromEquiv $ Reactor.Equivalent.symm u.equiv)
+    simp [fromEquiv] at h
 
 end StrictMember
 
@@ -110,16 +118,16 @@ variable [Hierarchical α] {rtr rtr₁ : α}
 theorem unique (m₁ m₂ : Member cpt i rtr) : m₁ = m₂ :=
   unique_ids.allEq m₁ m₂
 
-theorem rtr_equiv (e : rtr₁ ≈ rtr₂) : 
+theorem rtr_equiv (e : rtr₁ ≈ rtr₂) :
     (m₁ : Member .rtr i rtr₁) → (m₂ : Member .rtr i rtr₂) → m₁.object ≈ m₂.object
   | root,      root      => e
   | strict s₁, strict s₂ => s₁.rtr_equiv e s₂
 
 theorem equiv_rcn_eq (e : rtr₁ ≈ rtr₂) :
-    (m₁ : Member .rcn i rtr₁) → (m₂ : Member .rcn i rtr₂) → m₁.object = m₂.object 
+    (m₁ : Member .rcn i rtr₁) → (m₂ : Member .rcn i rtr₂) → m₁.object = m₂.object
   | strict s₁, strict s₂ => s₁.equiv_rcn_eq e s₂
 
-theorem lawfulMemUpdate_object_preserved 
+theorem lawfulMemUpdate_object_preserved
     (u : LawfulMemUpdate cpt i v rtr₁ rtr₂) (h : c ≠ cpt ∨ j ≠ i) :
     (m₁ : Member c j rtr₁) → (m₂ : Member c j rtr₂) → m₁.object = m₂.object
   | .strict s₁, .strict s₂ => s₁.lawfulMemUpdate_object_preserved u h s₂
@@ -136,24 +144,24 @@ theorem unique : (Object rtr cpt i o₁) → (Object rtr cpt i o₂) → o₁ = 
   | ⟨m₁⟩, ⟨m₂⟩ => m₁.unique m₂ ▸ rfl
 
 theorem iff_obj?_some : (Object rtr cpt i o) ↔ (rtr[cpt][i] = some o) where
-  mp := by 
+  mp := by
     intro ⟨m⟩
-    simp [obj?]
+    simp only [obj?]
     split
-    case inl h =>
+    case isTrue h =>
       have ⟨m', h'⟩ := Object.def.mp h.choose_spec
       simp [←h', m.unique m']
-    case inr h =>
+    case isFalse h =>
       push_neg at h
       specialize h m.object
       simp [Object.def] at h
   mpr h := by
-    simp [obj?] at h
+    simp only [obj?] at h
     split at h
-    case inr => contradiction
-    case inl h h' => 
+    case isFalse => contradiction
+    case isTrue h h' =>
       have ⟨m', h'⟩ := Object.def.mp h'.choose_spec
-      exact Option.some_inj.mp h ▸ h' ▸ ⟨m'⟩ 
+      exact Option.some_inj.mp h ▸ h' ▸ ⟨m'⟩
 
 theorem not_iff_obj?_none : (∀ o, ¬Object rtr cpt i o) ↔ (rtr[cpt][i] = none) := by
   simp [Option.eq_none_iff_forall_not_mem, iff_obj?_some]
@@ -166,27 +174,27 @@ namespace Hierarchical
 variable [Hierarchical α] {rtr : α}
 
 theorem get?_some_to_obj?_some (h : rtr{cpt}{i} = some o) : rtr[cpt][i] = some o :=
-  Object.iff_obj?_some.mp ⟨.final h⟩ 
+  Object.iff_obj?_some.mp ⟨.final h⟩
 
 theorem obj?_root_some (ho : rtr[.rtr][⊤] = some o) : o = rtr :=
   have ⟨m⟩ := Object.iff_obj?_some.mpr ho
   match m with | .root => rfl
 
--- Note: This theorem does not hold for `i' = ⊤`. For a version that supports this case see 
+-- Note: This theorem does not hold for `i' = ⊤`. For a version that supports this case see
 --       `obj?_some_nested'`.
-theorem obj?_some_nested {i' : ID} (h : rtr{.rtr}{i} = some rtr') (ho : rtr'[cpt][i'] = some o) : 
+theorem obj?_some_nested {i' : ID} (h : rtr{.rtr}{i} = some rtr') (ho : rtr'[cpt][i'] = some o) :
     rtr[cpt][i'] = some o := by
   have ⟨s, hs⟩ := Object.strict_elim $ Object.iff_obj?_some.mpr ho
-  exact Object.iff_obj?_some.mp $ hs ▸ ⟨.nested h s⟩ 
+  exact Object.iff_obj?_some.mp $ hs ▸ ⟨.nested h s⟩
 
-theorem obj?_some_nested' (h : rtr{.rtr}{i} = some rtr') (ho : rtr'[cpt][i'] = some o) : 
+theorem obj?_some_nested' (h : rtr{.rtr}{i} = some rtr') (ho : rtr'[cpt][i'] = some o) :
     ∃ j, rtr[cpt][j] = some o := by
   cases cpt <;> try cases i'
   case rtr.none =>
     exists i
-    exact Object.iff_obj?_some.mp $ obj?_root_some ho ▸ ⟨.final h⟩ 
-  all_goals 
-    exact ⟨_, obj?_some_nested h ho⟩ 
+    exact Object.iff_obj?_some.mp $ obj?_root_some ho ▸ ⟨.final h⟩
+  all_goals
+    exact ⟨_, obj?_some_nested h ho⟩
 
 theorem obj?_some_extend (ho : rtr[.rtr][c] = some con) (hc : con{cpt}{i} = some o) :
     rtr[cpt][i] = some o := by
@@ -194,7 +202,7 @@ theorem obj?_some_extend (ho : rtr[.rtr][c] = some con) (hc : con{cpt}{i} = some
   exact Object.iff_obj?_some.mp $ m.extend_object hc ▸ ⟨m.extend hc⟩
 
 -- Note: This theorem does not hold for `i = ⊤`.
-theorem obj?_some_split {i : ID} (ho : rtr[cpt][i] = some o) : 
+theorem obj?_some_split {i : ID} (ho : rtr[cpt][i] = some o) :
     ∃ c con, (rtr[.rtr][c] = some con) ∧ (con{cpt}{i} = some o) := by
   have ⟨s, hs⟩ := Object.strict_elim $ Object.iff_obj?_some.mpr ho
   have ⟨c, ⟨m, hm⟩⟩ := s.split'
@@ -203,20 +211,20 @@ theorem obj?_some_split {i : ID} (ho : rtr[cpt][i] = some o) :
 theorem member_isEmpty_obj?_none (h : IsEmpty $ Member cpt i rtr) : rtr[cpt][i] = none :=
   Object.not_iff_obj?_none.mp (Object.not_of_member_isEmpty h ·)
 
-theorem get?_some_rtr_eq (ho₁ : rtr[.rtr][c₁] = some con₁) (ho₂ : rtr[.rtr][c₂] = some con₂) 
+theorem get?_some_rtr_eq (ho₁ : rtr[.rtr][c₁] = some con₁) (ho₂ : rtr[.rtr][c₂] = some con₂)
     (hc₁ : con₁{cpt}{j} = some o₁) (hc₂ : con₂{cpt}{j} = some o₂) : c₁ = c₂ := by
   have ⟨m₁⟩ := Object.iff_obj?_some.mpr ho₁
   have ⟨m₂⟩ := Object.iff_obj?_some.mpr ho₂
-  exact Member.extend_inj $ (m₁.extend hc₁).unique (m₂.extend hc₂) 
-    
-theorem mem_get?_rtr_eq (ho₁ : rtr[.rtr][c₁] = some con₁) (ho₂ : rtr[.rtr][c₂] = some con₂) 
+  exact Member.extend_inj $ (m₁.extend hc₁).unique (m₂.extend hc₂)
+
+theorem mem_get?_rtr_eq (ho₁ : rtr[.rtr][c₁] = some con₁) (ho₂ : rtr[.rtr][c₂] = some con₂)
     (hc₁ : j ∈ con₁{cpt}) (hc₂ : j ∈ con₂{cpt}) : c₁ = c₂ :=
   get?_some_rtr_eq ho₁ ho₂ (Partial.mem_iff.mp hc₁).choose_spec (Partial.mem_iff.mp hc₂).choose_spec
 
 theorem obj?_none_to_get?_none {i : ID} (ho : rtr[cpt][i] = none) : rtr{cpt}{i} = none := by
   replace ho := Object.not_iff_obj?_none.mpr ho
   by_contra h
-  exact ho _ ⟨.final $ Option.ne_none_iff_exists.mp h |>.choose_spec.symm⟩ 
+  exact ho _ ⟨.final $ Option.ne_none_iff_exists.mp h |>.choose_spec.symm⟩
 
 end Hierarchical
 
@@ -233,7 +241,7 @@ theorem mem_iff {i} (e : rtr₁ ≈ rtr₂) : (i ∈ rtr₁[cpt]) ↔ (i ∈ rtr
   simp [Partial.mem_iff, obj?_some_iff e]
 
 theorem ids_eq (e : rtr₁ ≈ rtr₂) : rtr₁[cpt].ids = rtr₂[cpt].ids := by
-  ext1 
+  ext1
   exact mem_iff e
 
 theorem obj?_none_iff (e : rtr₁ ≈ rtr₂) : (rtr₁[cpt][i] = none) ↔ (rtr₂[cpt][i] = none) := by
@@ -245,7 +253,7 @@ theorem obj?_none_iff (e : rtr₁ ≈ rtr₂) : (rtr₁[cpt][i] = none) ↔ (rtr
   · exact Equivalent.symm e
   · exact e
 
-theorem obj?_rtr_equiv 
+theorem obj?_rtr_equiv
     (e : rtr₁ ≈ rtr₂) (h₁ : rtr₁[.rtr][i] = some n₁) (h₂ : rtr₂[.rtr][i] = some n₂) : n₁ ≈ n₂ := by
   have ⟨m₁⟩ := Object.iff_obj?_some.mpr h₁
   have ⟨m₂⟩ := Object.iff_obj?_some.mpr h₂
@@ -254,14 +262,14 @@ theorem obj?_rtr_equiv
 theorem obj?_rtr_equiv' (e : rtr₁ ≈ rtr₂) (h₂ : rtr₂[.rtr][i] = some n₂) :
     ∃ n₁, (rtr₁[.rtr][i] = some n₁) ∧ (n₁ ≈ n₂) := by
   have ⟨_, h₁⟩ := obj?_some_iff e |>.mpr ⟨_, h₂⟩
-  exact ⟨_, h₁, Equivalent.obj?_rtr_equiv e h₁ h₂⟩ 
+  exact ⟨_, h₁, Equivalent.obj?_rtr_equiv e h₁ h₂⟩
 
 theorem obj?_rcn_eq (e : rtr₁ ≈ rtr₂) : rtr₁[.rcn] = rtr₂[.rcn] := by
   funext i
   cases ho₁ : rtr₁[.rcn][i]
   case none => simp [obj?_none_iff e |>.mp ho₁]
   case some =>
-    have ⟨_, ho₂⟩ := obj?_some_iff e |>.mp ⟨_, ho₁⟩ 
+    have ⟨_, ho₂⟩ := obj?_some_iff e |>.mp ⟨_, ho₁⟩
     have ⟨m₁⟩ := Object.iff_obj?_some.mpr ho₁
     have ⟨m₂⟩ := Object.iff_obj?_some.mpr ho₂
     simp [ho₂, m₁.equiv_rcn_eq e m₂]
@@ -275,37 +283,37 @@ open Hierarchical
 variable [Hierarchical α] {rtr₁ : α}
 
 theorem obj?_some₁ (u : LawfulMemUpdate cpt i v rtr₁ rtr₂) : ∃ o, rtr₁[cpt][i] = some o := by
-  induction u 
+  induction u
   case final           => exact ⟨_, get?_some_to_obj?_some ‹_›⟩
   case nested h _ _ hi => exact ⟨_, obj?_some_nested h hi.choose_spec⟩
 
 theorem obj?_some₂ (u : LawfulMemUpdate cpt i v rtr₁ rtr₂) : ∃ o, rtr₂[cpt][i] = some o := by
-  induction u 
+  induction u
   case final         => exact ⟨_, get?_some_to_obj?_some ‹_›⟩
   case nested h _ hi => exact ⟨_, obj?_some_nested h hi.choose_spec⟩
 
-theorem obj?_some_iff (u : LawfulMemUpdate cpt i v rtr₁ rtr₂) : 
+theorem obj?_some_iff (u : LawfulMemUpdate cpt i v rtr₁ rtr₂) :
     (∃ o, rtr₁[c][j] = some o) ↔ (∃ o, rtr₂[c][j] = some o) :=
   Equivalent.obj?_some_iff u.equiv
 
-theorem obj?_none_iff (u : LawfulMemUpdate cpt i v rtr₁ rtr₂) : 
+theorem obj?_none_iff (u : LawfulMemUpdate cpt i v rtr₁ rtr₂) :
     (rtr₁[c][j] = none) ↔ (rtr₂[c][j] = none) :=
   Equivalent.obj?_none_iff u.equiv
 
-theorem obj?_preserved (u : LawfulMemUpdate cpt i v rtr₁ rtr₂) (h : c ≠ cpt ∨ j ≠ i) : 
+theorem obj?_preserved (u : LawfulMemUpdate cpt i v rtr₁ rtr₂) (h : c ≠ cpt ∨ j ≠ i) :
     rtr₂[c][j] = rtr₁[c][j] := by
   cases ho₁ : rtr₁[c][j]
   case none => simp [obj?_none_iff u |>.mp ho₁]
   case some =>
-    have ⟨_, ho₂⟩ := obj?_some_iff u |>.mp ⟨_, ho₁⟩ 
+    have ⟨_, ho₂⟩ := obj?_some_iff u |>.mp ⟨_, ho₁⟩
     have ⟨m₁⟩ := Object.iff_obj?_some.mpr ho₁
     have ⟨m₂⟩ := Object.iff_obj?_some.mpr ho₂
     simp [ho₂, m₁.lawfulMemUpdate_object_preserved u h m₂]
 
-theorem obj?_updated (u : LawfulMemUpdate cpt i v rtr₁ rtr₂) : 
+theorem obj?_updated (u : LawfulMemUpdate cpt i v rtr₁ rtr₂) :
     rtr₂[cpt][i] = (fun _ => v) <$> rtr₁[cpt][i] := by
   induction u
-  case final h₁ h₂ => 
+  case final h₁ h₂ =>
     rw [get?_some_to_obj?_some h₁, get?_some_to_obj?_some h₂, Option.map_some]
   case nested h₁ h₂ u hi =>
     have ⟨_, h₁'⟩ := u.obj?_some₁
@@ -321,12 +329,12 @@ namespace LawfulUpdate
 open Hierarchical
 variable [Hierarchical α] {rtr₁ : α}
 
-theorem obj?_preserved (h : c ≠ cpt ∨ j ≠ i) : 
+theorem obj?_preserved (h : c ≠ cpt ∨ j ≠ i) :
     (LawfulUpdate cpt i v rtr₁ rtr₂) → rtr₂[c][j] = rtr₁[c][j]
   | update u   => u.obj?_preserved h
   | notMem _ h => h ▸ rfl
 
-theorem obj?_updated : 
+theorem obj?_updated :
     (LawfulUpdate cpt i v rtr₁ rtr₂) → rtr₂[cpt][i] = (fun _ => v) <$> rtr₁[cpt][i]
   | update u   => u.obj?_updated
   | notMem h e => by subst e; simp [member_isEmpty_obj?_none h]
