ReactorModel/Objects/Reactor/Theorems/Proper.lean
@@ -16,19 +16,20 @@ namespace Wellformed
 open Hierarchical Equivalent
 variable [Hierarchical α] {rtr rtr₁ : α}
 
-scoped macro "equiv_local_proof " dep:ident : term => 
+local macro "equiv_local_proof " dep:ident : term =>
   `($dep $ mem_get?_iff (obj?_rtr_equiv ‹_› ‹_› ‹_›) |>.mp ‹_›)
 
-set_option hygiene false in
-scoped macro "equiv_nested_proof " dep:ident : term => `(
-  fun hc hp => 
+set_option hygiene false in section
+
+local macro "equiv_nested_proof " dep:ident : term => `(
+  fun hc hp =>
     have e        := obj?_rtr_equiv ‹_› h₁ h₂
-    have ⟨_, hc'⟩ := get?_some_iff e |>.mp ⟨_, hc⟩ 
+    have ⟨_, hc'⟩ := get?_some_iff e |>.mp ⟨_, hc⟩
     $dep hc' $ (mem_get?_iff $ get?_rtr_some_equiv e hc hc').mp hp
 )
 
-theorem ValidDependency.equiv 
-    (e : rtr₁ ≈ rtr₂) (h₁ : rtr₁[.rtr][j] = some con₁) (h₂ : rtr₂[.rtr][j] = some con₂) : 
+theorem ValidDependency.equiv
+    (e : rtr₁ ≈ rtr₂) (h₁ : rtr₁[.rtr][j] = some con₁) (h₂ : rtr₂[.rtr][j] = some con₂) :
     (ValidDependency con₁ rk dk d) → ValidDependency con₂ rk dk d
   | inp h           => equiv_local_proof inp
   | out h           => equiv_local_proof out
@@ -37,13 +38,15 @@ theorem ValidDependency.equiv
   | nestedIn  hc hp => (equiv_nested_proof nestedIn) hc hp
   | nestedOut hc hp => (equiv_nested_proof nestedOut) hc hp
 
+end
+
 theorem equiv (e : rtr₁ ≈ rtr₂) (wf : Wellformed rtr₁) : Wellformed rtr₂ where
-  unique_inputs h₁ h₂ := 
+  unique_inputs h₁ h₂ :=
     wf.unique_inputs (e.obj?_rcn_eq.symm ▸ h₁) (e.obj?_rcn_eq.symm ▸ h₂)
-  ordered_prio h₁ h₂ h₃ := 
+  ordered_prio h₁ h₂ h₃ :=
     have ⟨_, h₁', e⟩ := Equivalent.obj?_rtr_equiv' e h₁
     ordered_prio ‹_› h₁' (get?_rcn_eq e ▸ h₂) (get?_rcn_eq e ▸ h₃)
-  valid_deps h₁ h₂ h₃ := 
+  valid_deps h₁ h₂ h₃ :=
     have ⟨_, h₁', e⟩ := Equivalent.obj?_rtr_equiv' e h₁
     wf.valid_deps h₁' (get?_rcn_eq e ▸ h₂) h₃ |>.equiv ‹_› h₁' h₁
 
@@ -51,22 +54,23 @@ theorem nested (wf : Wellformed rtr₁) (h : rtr₁{.rtr}{i} = some rtr₂) : We
   unique_inputs h₁ h₂ := wf.unique_inputs (obj?_some_nested h h₁) (obj?_some_nested h h₂)
   ordered_prio h₁     := wf.ordered_prio (obj?_some_nested' h h₁).choose_spec
   valid_deps h₁       := wf.valid_deps (obj?_some_nested' h h₁).choose_spec
-  
-variable (wf : Wellformed rtr)
 
-theorem shared_dep_local 
+variable (wf : Wellformed rtr)
+include wf
+
+theorem shared_dep_local
     (hc₁ : rtr[.rtr][c₁] = some con₁) (hc₂ : rtr[.rtr][c₂] = some con₂)
     (hr₁ : con₁{.rcn}{i₁} = some rcn₁) (hr₂ : con₂{.rcn}{i₂} = some rcn₂)
-    (hd₁ : ⟨cpt, j⟩ ∈ rcn₁.deps k) (hd₂ : ⟨cpt, j⟩ ∈ rcn₂.deps k) : 
+    (hd₁ : ⟨cpt, j⟩ ∈ rcn₁.deps k) (hd₂ : ⟨cpt, j⟩ ∈ rcn₂.deps k) :
     c₁ = c₂ := by
   by_cases hi : i₁ = i₂
   case pos => exact get?_some_rtr_eq hc₁ hc₂ (hi ▸ hr₁) hr₂
   case neg =>
     have hv₁ := wf.valid_deps hc₁ hr₁ hd₁
     have hv₂ := wf.valid_deps hc₂ hr₂ hd₂
-    cases k <;> cases cpt <;> try cases ‹Kind› 
+    cases k <;> cases cpt <;> try cases ‹Kind›
     have := obj?_some_extend hc₁ hr₁
-    case out.inp => 
+    case out.inp =>
       have hd₂' := wf.unique_inputs (obj?_some_extend hc₁ hr₁) (obj?_some_extend hc₂ hr₂) hi hd₁
       exact absurd hd₂ hd₂'
     case in.out =>
@@ -76,27 +80,27 @@ theorem shared_dep_local
         have hc₂' := obj?_some_extend hc₂ hn₂
         have hj := mem_get?_rtr_eq hc₁' hc₂' hj₁ hj₂
         injection hj with hj
-        exact get?_some_rtr_eq hc₁ hc₂ (hj ▸ hn₁) hn₂ 
-    all_goals 
+        exact get?_some_rtr_eq hc₁ hc₂ (hj ▸ hn₁) hn₂
+    all_goals
       cases hk₁ : rcn₁.kind <;> cases hk₂ : rcn₂.kind <;> cases hk₁ ▸ hv₁ <;> cases hk₂ ▸ hv₂
-      all_goals exact mem_get?_rtr_eq hc₁ hc₂ ‹_› ‹_› 
-        
+      all_goals exact mem_get?_rtr_eq hc₁ hc₂ ‹_› ‹_›
+
 theorem shared_state_local
     (hc₁ : rtr[.rtr][c₁] = some con₁) (hc₂ : rtr[.rtr][c₂] = some con₂)
-    (hr₁ : con₁{.rcn}{i₁} = some rcn₁) (hr₂ : con₂{.rcn}{i₂} = some rcn₂) 
-    (hd₁ : ⟨.stv, j⟩ ∈ rcn₁.deps k₁) (hd₂ : ⟨.stv, j⟩ ∈ rcn₂.deps k₂) : 
+    (hr₁ : con₁{.rcn}{i₁} = some rcn₁) (hr₂ : con₂{.rcn}{i₂} = some rcn₂)
+    (hd₁ : ⟨.stv, j⟩ ∈ rcn₁.deps k₁) (hd₂ : ⟨.stv, j⟩ ∈ rcn₂.deps k₂) :
     c₁ = c₂ := by
   have hv₁ := wf.valid_deps hc₁ hr₁ hd₁
   have hv₂ := wf.valid_deps hc₂ hr₂ hd₂
   cases hk₁ : rcn₁.kind <;> cases hk₂ : rcn₂.kind <;> cases hk₁ ▸ hv₁ <;> cases hk₂ ▸ hv₂
-  all_goals exact mem_get?_rtr_eq hc₁ hc₂ ‹_› ‹_› 
+  all_goals exact mem_get?_rtr_eq hc₁ hc₂ ‹_› ‹_›
 
 end Wellformed
 
 open Hierarchical in
-theorem ext_obj? [Proper α] {rtr₁ : α} (e : rtr₁ ≈ rtr₂) 
-    (h : ∀ {c : Component.Valued} {i o₁ o₂}, 
-          (rtr₁[c][i] = some o₁) → (rtr₂[c][i] = some o₂) → o₁ = o₂) : 
+theorem ext_obj? [Proper α] {rtr₁ : α} (e : rtr₁ ≈ rtr₂)
+    (h : ∀ {c : Component.Valued} {i o₁ o₂},
+          (rtr₁[c][i] = some o₁) → (rtr₂[c][i] = some o₂) → o₁ = o₂) :
     rtr₁ = rtr₂ := by
   induction rtr₁ using WellFounded.induction generalizing rtr₂
   case nested rtr₁ hi =>
@@ -105,7 +109,7 @@ theorem ext_obj? [Proper α] {rtr₁ : α} (e : rtr₁ ≈ rtr₂)
       cases hc₁ : rtr₁{cpt}{i}
       case none => simp [Equivalent.get?_none_iff e |>.mp hc₁]
       case some n₁ =>
-        have ⟨n₂, hc₂⟩ := Equivalent.get?_some_iff e |>.mp ⟨_, hc₁⟩ 
+        have ⟨n₂, hc₂⟩ := Equivalent.get?_some_iff e |>.mp ⟨_, hc₁⟩
         simp [hc₂]
         cases cpt
         case rcn => exact Equivalent.get?_rcn_some_eq e hc₁ hc₂
@@ -113,14 +117,14 @@ theorem ext_obj? [Proper α] {rtr₁ : α} (e : rtr₁ ≈ rtr₂)
           apply hi n₁ ⟨_, hc₁⟩ $ Equivalent.get?_rtr_some_equiv e hc₁ hc₂
           intro c _ _ _ ho₁ ho₂
           exact h (obj?_some_nested hc₁ ho₁) (obj?_some_nested hc₂ ho₂)
-        all_goals 
+        all_goals
           have ho₁ := get?_some_to_obj?_some hc₁
           have ho₂ := get?_some_to_obj?_some hc₂
           exact h ho₁ ho₂
-        
-theorem LawfulUpdate.ne_comm [Proper α] {rtr rtr₁ rtr₁' rtr₂ rtr₂' : α} 
-    (u₁ : LawfulUpdate cpt₁ i₁ v₁ rtr rtr₁) (u₂ : LawfulUpdate cpt₂ i₂ v₂ rtr₁ rtr₂) 
-    (u₁' : LawfulUpdate cpt₂ i₂ v₂ rtr rtr₁') (u₂' : LawfulUpdate cpt₁ i₁ v₁ rtr₁' rtr₂') 
+
+theorem LawfulUpdate.ne_comm [Proper α] {rtr rtr₁ rtr₁' rtr₂ rtr₂' : α}
+    (u₁ : LawfulUpdate cpt₁ i₁ v₁ rtr rtr₁) (u₂ : LawfulUpdate cpt₂ i₂ v₂ rtr₁ rtr₂)
+    (u₁' : LawfulUpdate cpt₂ i₂ v₂ rtr rtr₁') (u₂' : LawfulUpdate cpt₁ i₁ v₁ rtr₁' rtr₂')
     (h : cpt₁ ≠ cpt₂ ∨ i₁ ≠ i₂) : rtr₂ = rtr₂' := by
   have e₁ := Equivalent.trans u₁.equiv u₂.equiv
   have e₂ := Equivalent.trans u₁'.equiv u₂'.equiv
@@ -132,33 +136,33 @@ theorem LawfulUpdate.ne_comm [Proper α] {rtr rtr₁ rtr₁' rtr₂ rtr₂' : α
   by_cases hc₁ : cpt = cpt₁ <;> by_cases hc₂ : cpt = cpt₂ <;> ((try subst hc₁); try subst hc₂)
   · by_cases hi₁ : i = i₁ <;> by_cases hi₂ : i = i₂ <;> ((try subst hi₁); try subst hi₂)
     · simp at h
-    · have h₁ := u₁.obj?_updated ▸ u₂.obj?_preserved (.inr hi₂) 
-      have h₂ := u₁'.obj?_preserved (.inr hi₂) ▸ u₂'.obj?_updated  
+    · have h₁ := u₁.obj?_updated ▸ u₂.obj?_preserved (.inr hi₂)
+      have h₂ := u₁'.obj?_preserved (.inr hi₂) ▸ u₂'.obj?_updated
       injection ho₁ ▸ h₂.trans h₁.symm ▸ ho₂
     · have h₁ := u₁.obj?_preserved (.inr hi₁) ▸ u₂.obj?_updated
       have h₂ := u₁'.obj?_updated ▸ u₂'.obj?_preserved (.inr hi₁)
       injection ho₁ ▸ h₂.trans h₁.symm ▸ ho₂
-    · have := u₁.obj?_preserved  (.inr hi₁) ▸ u₂.obj?_preserved  (.inr hi₂) 
+    · have := u₁.obj?_preserved  (.inr hi₁) ▸ u₂.obj?_preserved  (.inr hi₂)
       have := u₁'.obj?_preserved (.inr hi₂) ▸ u₂'.obj?_preserved (.inr hi₁)
       simp_all
   · by_cases hi₁ : i = i₁ <;> try subst hi₁
-    · have h₁ := u₁.obj?_updated ▸ u₂.obj?_preserved (.inl hc₂) 
-      have h₂ := u₁'.obj?_preserved (.inl hc₂) ▸ u₂'.obj?_updated  
+    · have h₁ := u₁.obj?_updated ▸ u₂.obj?_preserved (.inl hc₂)
+      have h₂ := u₁'.obj?_preserved (.inl hc₂) ▸ u₂'.obj?_updated
       injection ho₁ ▸ h₂.trans h₁.symm ▸ ho₂
-    · have := u₁.obj?_preserved  (.inr hi₁) ▸ u₂.obj?_preserved (.inl hc₂) 
+    · have := u₁.obj?_preserved  (.inr hi₁) ▸ u₂.obj?_preserved (.inl hc₂)
       have := u₁'.obj?_preserved (.inl hc₂) ▸ u₂'.obj?_preserved (.inr hi₁)
       simp_all
   · by_cases hi₂ : i = i₂ <;> try subst hi₂
-    · have h₁ := u₁.obj?_preserved (.inl hc₁) ▸ u₂.obj?_updated 
-      have h₂ := u₁'.obj?_updated ▸ u₂'.obj?_preserved (.inl hc₁)  
+    · have h₁ := u₁.obj?_preserved (.inl hc₁) ▸ u₂.obj?_updated
+      have h₂ := u₁'.obj?_updated ▸ u₂'.obj?_preserved (.inl hc₁)
       injection ho₁ ▸ h₂.trans h₁.symm ▸ ho₂
-    · have := u₁.obj?_preserved  (.inl hc₁) ▸ u₂.obj?_preserved (.inr hi₂) 
+    · have := u₁.obj?_preserved  (.inl hc₁) ▸ u₂.obj?_preserved (.inr hi₂)
       have := u₁'.obj?_preserved (.inr hi₂) ▸ u₂'.obj?_preserved (.inl hc₁)
       simp_all
-  · have := u₁.obj?_preserved  (j := i) (.inl hc₁) ▸ u₂.obj?_preserved  (.inl hc₂) 
+  · have := u₁.obj?_preserved  (j := i) (.inl hc₁) ▸ u₂.obj?_preserved  (.inl hc₂)
     have := u₁'.obj?_preserved (j := i) (.inl hc₂) ▸ u₂'.obj?_preserved (.inl hc₁)
     simp_all
-  
+
 open Updatable in
 theorem LawfulUpdatable.update_ne_comm [Proper α] {rtr : α} (h : cpt₁ ≠ cpt₂ ∨ i₁ ≠ i₂):
     update (update rtr cpt₁ i₁ v₁) cpt₂ i₂ v₂ = update (update rtr cpt₂ i₂ v₂) cpt₁ i₁ v₁ :=
