ReactorModel/Primitives.lean
@@ -9,10 +9,10 @@ private opaque PresentValue : Type
 
 -- `Value`s are the objects that are consumed and produced by reactions
 -- and passed along via ports and actions.
--- The `absent` value is a special value which is used with ports to 
+-- The `absent` value is a special value which is used with ports to
 -- represent that a given port is not populated with a value.
-inductive Value 
-  | absent 
+inductive Value
+  | absent
   | present (val : PresentValue)
 
 inductive Value.IsPresent : Value → Prop
@@ -24,7 +24,7 @@ opaque ID : Type
 
 -- Note: This approach is also used in the implementation of Lean:
 --       https://github.com/leanprover/lean4/blob/b81cff/src/Lean/Environment.lean#L18
-opaque PrioritySpec : (p : Type) × (PartialOrder p) := ⟨Unit, inferInstance⟩ 
+opaque PrioritySpec : (p : Type) × (PartialOrder p) := ⟨Unit, inferInstance⟩
 
 -- The `Priority` type is used to impose a (potentially partial) order on reactions.
 def Priority := PrioritySpec.fst
@@ -33,9 +33,9 @@ instance : PartialOrder Priority := PrioritySpec.snd
 
 -- The `Kind` type is used to generically distinguish between things which
 -- have an "input" and "output" variant. This is the case for ports as well
--- as ports' dependencies. 
+-- as ports' dependencies.
 inductive Kind
-  | «in» 
+  | «in»
   | out
 deriving DecidableEq
 
@@ -54,10 +54,10 @@ instance : OfNat Time 0 where
 -- A `Time.Tag` is used to represent a logical time tag.
 -- The order of these tags is lexicographical with the `time` taking priority.
 @[ext]
-structure Time.Tag where 
+structure Time.Tag where
   time : Time
   microstep : Nat
-  
+
 namespace Time.Tag
 
 instance : LE Time.Tag where
@@ -70,19 +70,19 @@ instance : LinearOrder Time.Tag where
   le_trans _ _ _
     | .inl h₁, .inl h₂ => .inl $ h₁.trans h₂
     | .inl h₁, .inr ⟨h₂, _⟩ | .inr ⟨h₂, _⟩, .inl h₁ => .inl $ h₂ ▸ h₁
-    | .inr ⟨h₁, h₁'⟩, .inr ⟨h₂, h₂'⟩ => .inr ⟨h₁.trans h₂, h₁'.trans h₂'⟩ 
+    | .inr ⟨h₁, h₁'⟩, .inr ⟨h₂, h₂'⟩ => .inr ⟨h₁.trans h₂, h₁'.trans h₂'⟩
   le_antisymm := by
     intro _ _; intro
     | .inl h₁, .inl h₂ => exact absurd h₁ h₂.asymm
     | .inl h₁, .inr ⟨h₂, _⟩ | .inr ⟨h₂, _⟩, .inl h₁ => exact absurd (h₂ ▸ h₁) (lt_irrefl _)
-    | .inr ⟨h₁, h₁'⟩, .inr ⟨h₂, h₂'⟩ => exact Time.Tag.ext _ _ (h₁ ▸ h₂) (h₁'.antisymm h₂') 
-  le_total := by 
+    | .inr ⟨h₁, h₁'⟩, .inr ⟨h₂, h₂'⟩ => exact Time.Tag.ext (h₁ ▸ h₂) (h₁'.antisymm h₂')
+  le_total := by
     intro ⟨t₁, m₁⟩ ⟨t₂, m₂⟩
     by_cases ht : t₁ = t₂ <;> by_cases hm : m₁ = m₂ <;> simp_all
-    · exact .inr ⟨rfl, le_rfl⟩ 
+    · exact .inr ⟨rfl, le_rfl⟩
     · cases Nat.le_total m₁ m₂
       · exact .inl $ .inr ⟨rfl, ‹_›⟩
-      · exact .inr $ .inr ⟨rfl, ‹_›⟩  
+      · exact .inr $ .inr ⟨rfl, ‹_›⟩
     all_goals
       cases Nat.le_total t₁ t₂
       · exact .inl $ .inl $ lt_of_le_of_ne ‹_› ht
@@ -91,8 +91,6 @@ instance : LinearOrder Time.Tag where
   decidableEq := inferInstance
 
 instance : OfNat Time.Tag 0 where
-  ofNat := ⟨0, 0⟩ 
+  ofNat := ⟨0, 0⟩
 
-end Time.Tag  
-
-
+end Time.Tag
