lakefile.lean
@@ -1,7 +1,0 @@
-import Lake
-open Lake DSL
-
-package reactor_model
-lean_lib ReactorModel
-
-require mathlib from git "https://github.com/leanprover-community/mathlib4.git"@"v4.7.0-rc2"
