README.md
@@ -4,14 +4,8 @@ This repository contains a [Lean](https://github.com/leanprover/lean4)-based for
 
 ## Resources
 
-While this formalization differs quite significantly from previous work, the following list contains relevant literature covering the Reactor model.
+The paper [Provable Determinism for Software in Cyber-Physical Systems](https://cfaed.tu-dresden.de/files/Images/people/chair-cc/publications/2310_Rossel_VSSTE.pdf) explains the formalization at a high level. While this formalization differs quite significantly from previous work, the following list contains relevant literature covering the Reactor model:
 
 * [Reactors: A Deterministic Model of Concurrent Computation for Reactive Systems (Lohstroh 2020)](https://www2.eecs.berkeley.edu/Pubs/TechRpts/2020/EECS-2020-235.pdf)
 * [Reactors: A Deterministic Model for Composable Reactive Systems (Lohstroh et al. 2019)](https://ptolemy.berkeley.edu/publications/papers/19/Lohstroh_etAl_Reactor_CyPhy19_PDFA.pdf)
 * [List of related publications by the Lingua Franca community](https://www.lf-lang.org/publications-and-presentations)
-
-## Project Structure
-
-`ReactorModel/Objects` contains definitions and proofs about reactor objects.
-
-`ReactorModel/Execution` contains definitions and proofs for the execution model. Notably `Execution/Theorems/Execution.lean` contains the theorem of determinism and `Execution/Theorems/Progress.lean` the progress theorem.
